 Consider a parametrized curve in an oriented coordinate system, $(O,\Vector{i},\Vector{j})$:
 
 \[
  \Vector{r}(t)=
  \begin{pmatrix}
   x(t)\\y(t)
  \end{pmatrix},
 \]

 with $t$ in some interval, $I \subset \mathbb{R}$. We will assume that the functions $x(t)$ and $y(t)$ are two times
 diferentiable in $I$, ensuring the existence of the \emph{velocity}, $\Vector{v}(t)$, and \emph{acceleration}, $\Vector{a}(t)$, vectors:
 
 \[
  \Vector{v}(t)=
  \Vector{r}'(t)=
  \begin{pmatrix}
   x'(t)\\y'(t)
  \end{pmatrix},
  \qquad \qquad
  \Vector{a}(t)=
  \Vector{r}''(t)=
  \begin{pmatrix}
   x''(t)\\y''(t)
  \end{pmatrix}
 \]

%%\input{Introduction/Taylor}
 
The (scalar) velocity is given by:

\[
 v(t)=|\Vector{r}'(t)|=\sqrt{x'^2+y'^2}
\]

 A point of the curve where: $v(t) \neq 0$ is said to be \emph{regular}, in such a point we defined
 the unit tangent vector:
 
 \[
  \Vector{t}(t)=
  \frac{ \Vector{r}'(t) }{ |\Vector{r}'(t)| }
  =
  \frac{1
  }
  { \sqrt{ x'^2+y'^2} }
  \begin{pmatrix}
   x'\\y'
  \end{pmatrix},
 \]
 
 as well as it's positive normal:
 
 \[
  \Vector{n}(t)=
  \Vector{\widehat{t}}(t)=
  \frac{
  1
  }
  { \sqrt{ x'^2+y'^2} }
  \begin{pmatrix}
   -y'\\x'
  \end{pmatrix}
  \]

  Before we continue, we note that for a vector function of fixed length: $\Vector{a}(t) \cdot \Vector{a}(t)=l^2$,
  it's derivative is always perpendicular to itself:
  
  \[
   \Vector{a}(t) \cdot \Vector{a}'(t)=0
  \]

  In the following, we shall also need the unity vectors:
  
  \[
   \Vector{e}(t)=
  \begin{pmatrix}
   \cos{t}\\\sin{t}
  \end{pmatrix},
  \qquad 
   \Vector{f}(t)=
  \begin{pmatrix}
   -\sin{t}\\\cos{t}
  \end{pmatrix};
  \qquad   \qquad   
  \Vector{p}(t)=
  \begin{pmatrix}
   \sin{t}\\\cos{t}
  \end{pmatrix},
  \qquad
   \Vector{q}(t)=
  \begin{pmatrix}
   \cos{t}\\-\sin{t}
  \end{pmatrix}
  \]

Note that:

\[
 \Vector{ \widehat{e} }(t) =\Vector{f}(t),
 \qquad 
 \Vector{\widehat{f}}(t)=-\Vector{e}(t);
 \qquad \qquad
 \Vector{ \widehat{p} }(t) =\Vector{q}(t),
 \qquad 
 \Vector{\widehat{q}}(t)=-\Vector{p}(t)
\]

and:

\[
 \Vector{e}'(t) =\Vector{f}(t),
 \qquad 
 \Vector{f}'(t)=-\Vector{e}(t);
 \qquad \qquad
 \Vector{p}'(t) =-\Vector{q}(t),
 \qquad
 \Vector{q}'(t)=-\Vector{p}(t)
\]


