
Seja $\Vector{e}(t)$ um vetor \emph{normalizado}:
\[
 \Vector{e} \cdot \Vector{e} =1 
 \qquad \Rightarrow\qquad
 2\Vector{e} \cdot \Vector{e}'=0
 \qquad \Leftrightarrow\qquad
 \Vector{e} \perp \Vector{e}'
\]

Usaremos:

\[
 \Vector{e}(t)
 =
 \begin{pmatrix}
  \cos{t}\\\sin{t}
 \end{pmatrix}
  \qquad\qquad
 \Vector{f}(t)
 =
 \begin{pmatrix}
  -\sin{t}\\\cos{t}
 \end{pmatrix}  
\]

E:

\[
 \Vector{e} \cdot \Vector{e}=\Vector{f} \cdot \Vector{f}=1
 \qquad\qquad
  \Vector{e} \cdot \Vector{f}=0
\]

Notamos:

\[
 \Vector{ \widehat{e} } =\Vector{f}
 \qquad
  \Vector{ \widehat{f} } =-\Vector{e}
\]


Para seus derivados:

\[
 \Vector{e}'=\Vector{f}
 \qquad\qquad
 \Vector{f}'=-\Vector{e}
\]

No mais:

\[
 \Vector{e}_\omega(t)
 =
 \begin{pmatrix}
  \cos{\omega t}\\\sin{\omega t}
 \end{pmatrix}
  \qquad\qquad
 \Vector{f}_\omega(t)
 =
 \begin{pmatrix}
  -\sin{\omega t}\\\cos{\omega t}
 \end{pmatrix}  
\]

Novamente:

\[
\qquad
 \Vector{ \widehat{e} }_\omega =\Vector{f}_\omega
 \qquad
 \Vector{ \widehat{f} }_\omega =-\Vector{e}_\omega
 \qquad
\]

E:

\[
 \Vector{e}_\omega \cdot \Vector{e}_\omega=\Vector{f}_\omega \cdot \Vector{f}_\omega=1
 \qquad\qquad
  \Vector{e}_\omega \cdot \Vector{f}_\omega=0
\]

Por√©m,pela regra da cadeia:

\[
  \Vector{e}_\omega'=\omega\Vector{f}_\omega
 \qquad\qquad
 \Vector{f}_\omega'=-\omega\Vector{e}_\omega
\]

Para os produtos escalares:

\[
 \Vector{e} \cdot \Vector{e}_\omega
 =
 \Vector{f} \cdot \Vector{f}_\omega
 =
 \cos{t}\cos{\omega t}+\sin{t}\sin{\omega t}
 =
 \cos{ (\omega-1) t }
\]
