 In order to improve our approximation of the curve, we include second order derivatives:
 
 \[
  \label{eq:taylor:1}
  \Vector{r}(t)
  \approx
  \Vector{r}(t_0)
  +
  \Vector{r}'(t_0)(t-t_0)
  +
  \frac{1}{2}
  \Vector{r}''(t_0)(t-t_0)^2
\]

Since:

\[
 \Vector{r}'
 =
 v \Vector{t}
\]

we obtain:

\[
 \Vector{r}''
 =
 v' \Vector{t}
 +
 v \Vector{t}'
\]

Equivalently:

\[
 v \Vector{t}'
 =
 \Vector{r}''
 -
 v' \Vector{t}
\]

In a regular point of the curve:

\[
 \Vector{t}'
 =
 \frac{ \Vector{r}'' }{ v}
 -
 \frac{v'}{v} \Vector{t}
\]

