
 By \textbf{Taylors Formula}, we have for $t,t_0 \in I$:
 
 \begin{equation}
 \label{eq:taylor:n}
  \Vector{r}(t)
  =
  \Vector{r}(t_0)
  +
  \Vector{r}'(t_0)(t-t_0)
  +
  \ldots+
  \frac{1}{n!} \Vector{r}^{(n)}(t_0)(t-t_0)^n
  +
  \Vector{\epsilon}_n(t)
 \end{equation}
 
 In fact, Taylors Formula ensures, that for $t>t_0$, $\exists \xi \in [t_0,t]$, so that:
 
 \[
   |\Vector{\epsilon}_n(t)|
   \leq 
   \frac{1}{(n+1)!}
   |\Vector{r}^{(n+1)}(\xi)|(t-t_0)^{n+1}
 \]
 
Hence, for the \emph{Error Vector}, $\Vector{\epsilon}(t)$, we have:
 
\begin{equation}
  \lim_{t\rightarrow t_0} \frac{\Vector{\epsilon}_n(t)}{ (t-t_0)^n }
 \label{eq:taylor:err:n}
  =
  \Vector{0}
\end{equation}
 
\subsection{First Order Aproximation}
input{Introduction/First}
Deriving:

\[
 v(t)=\sqrt{ x'(t)^2+y'(t)^2},
\]

we observe:

\[
  v'(t)
  =
  \frac{x'(t)+y'(t)}{ \sqrt{ x'(t)^2+y'(t)^2} }
  =
  \frac{x'(t)+y'(t)}{ v }
\]


\subsection{Second Order Aproximation}
\input{Introduction/Second}
 

 